checkpoint

new/log.v
@@ -272,15 +272,3 @@ Proof.
 Qed.
 Hint Rewrite fl_log_cl_log_relationship.
 
-Fixpoint nlogn n : nat :=
-  match n with
-    | 0 => 0
-    | S n' => nlogn n' + (fl_log n' + 1)
-  end.
-
-Example nlogn_ex :
-  map nlogn (1 :: 2 :: 3 :: 4 ::  5 ::  6 ::  7 ::  8 ::  9 :: 10 :: nil)
-  = (1 :: 3 :: 5 :: 8 :: 11 :: 14 :: 17 :: 21 :: 25 :: 29 :: nil).
-Proof.
-  auto.
-Qed.
